Assert state-agreement in do_eval_oracle
Add the same assertion, that the next oracle state will agree
with the compiler output state, to the oracle generation process.
This should then meet up with the matching assertions in flatSem,
closSem etc.

compiler/backend/proofs/source_evalProofScript.sml
@@ -986,6 +986,7 @@ End
 
 Theorem elim_Case:
   (Case X /\ Y) = Y /\
+  (Y /\ Case X) = Y /\
   (Case X ==> Y) = Y
 Proof
   simp [Case_def]
@@ -1345,8 +1346,8 @@ Definition do_eval_oracle_def:
       let (env_id, st_v, decs) = orac 0 in
       (case compiler (env_id, st_v, decs), v_to_word8_list bs_v,
             v_to_word64_list ws_v of
-        | (SOME (_, c_bs, c_ws), SOME bs, SOME ws) =>
-            if bs = c_bs /\ ws = c_ws
+        | (SOME (st_v2, c_bs, c_ws), SOME bs, SOME ws) =>
+            if bs = c_bs /\ ws = c_ws /\ st_v2 (FST (SND (orac 1)))
             then SOME (env_id, shift_seq 1 orac, decs)
             else NONE
         | _ => NONE
@@ -1367,6 +1368,13 @@ Definition orac_agrees_def:
     | SOME (EvalOracle s) =>
       (!j. j < FST (FST (s.oracle 0)) ==> orac j = s.oracle (j + 1))
     | _ => F
+End
+
+(* the infinite extension of an oracle is still well-formed with
+   respect to the compiler function *)
+Definition orac_extended_wf_def:
+  orac_extended_wf (comp_f : compiler_fun) orac =
+  (!i x. comp_f (orac i) = SOME x ==> FST x (FST (SND (orac (SUC i)))))
 End
 
 Definition record_forward_def:
@@ -1418,9 +1426,12 @@ Theorem insert_do_eval:
   is_record f init_s es ==>
   is_record f init_s es' /\
   record_forward es es' /\
-  (orac_agrees orac es' ==>
+  (orac_agrees orac es' /\
+  orac_extended_wf f orac ==>
   do_eval vs (insert_oracle f orac es) = SOME (env, decs,
-    insert_oracle f orac es'))
+    insert_oracle f orac es')) /\
+  (recorded_orac_wf f (orac_s es).oracle ==>
+    recorded_orac_wf f (orac_s es').oracle)
 Proof
   simp [is_record_def, Once do_eval_def]
   \\ disch_tac
@@ -1430,12 +1441,25 @@ Proof
   \\ fs [do_eval_record_def, list_case_eq, option_case_eq] \\ rveq \\ fs []
   \\ rpt (pairarg_tac \\ fs [])
   \\ fs [COND_EXPAND_IMP]
-  \\ fs [compiler_agrees_def]
+  \\ every_case_tac \\ fs []
+  \\ imp_res_tac compiler_agrees_def
   \\ every_case_tac \\ fs []
   \\ simp [do_eval_oracle_def]
   \\ rveq \\ fs []
   \\ fs [record_forward_def, orac_agrees_def, shift_seq_def]
-  \\ Cases_on `env_id` \\ fs [lookup_env_def]
+  \\ rw []
+  >- (
+    fs [orac_extended_wf_def]
+    \\ rpt (first_x_assum (qspec_then `i` mp_tac))
+    \\ simp [ADD1]
+  )
+  >- (
+    Cases_on `env_id` \\ fs [lookup_env_def]
+  )
+  >- (
+    drule_then drule recorded_orac_wf_step
+    \\ simp []
+  )
 QED
 
 Theorem insert_declare_env:
@@ -1445,14 +1469,16 @@ Theorem insert_declare_env:
   record_forward es1 es2 /\
   (orac_agrees orac es2 ==>
   declare_env (insert_oracle f orac es1) env = SOME (x,
-    insert_oracle f orac es2))
+    insert_oracle f orac es2)) /\
+  (recorded_orac_wf f (orac_s es1).oracle ==>
+    recorded_orac_wf f (orac_s es2).oracle)
 Proof
   simp [is_record_def, declare_env_def, insert_oracle_def]
   \\ every_case_tac \\ fs []
   \\ disch_tac
   \\ fs [] \\ rveq \\ fs []
   \\ simp [PULL_EXISTS]
-  \\ simp [record_forward_def]
+  \\ simp [record_forward_def, recorded_orac_wf_def]
 QED
 
 Theorem reset_env_generation_orac_eqs:
@@ -1462,7 +1488,8 @@ Theorem reset_env_generation_orac_eqs:
   (reset_env_generation (insert_oracle f orac es1) es2 =
     reset_env_generation es1 es2) ∧
   (reset_env_generation es1 (insert_oracle f orac es2) =
-    insert_oracle f orac (reset_env_generation es1 es2))
+    insert_oracle f orac (reset_env_generation es1 es2)) ∧
+  ((orac_s (reset_env_generation es2 es3)).oracle = (orac_s es3).oracle)
 Proof
   simp [is_record_def, reset_env_generation_def, insert_oracle_def]
   \\ every_case_tac \\ fs []
@@ -1475,32 +1502,52 @@ Triviality record_forward_trans_sym
 Theorem evaluate_is_record_forward:
   (! ^s env exps s' res.
   evaluate s env exps = (s', res) /\
+  Case exps /\
   is_record f init_s s.eval_state
   ==>
   is_record f init_s s'.eval_state /\
-  record_forward s.eval_state s'.eval_state)
+  record_forward s.eval_state s'.eval_state /\
+  (recorded_orac_wf f (orac_s s.eval_state).oracle ==>
+    recorded_orac_wf f (orac_s s'.eval_state).oracle)
+  )
   /\
   (! ^s env x pes err_x s' res.
   evaluate_match s env x pes err_x = (s', res) /\
   is_record f init_s s.eval_state
   ==>
   is_record f init_s s'.eval_state /\
-  record_forward s.eval_state s'.eval_state)
+  record_forward s.eval_state s'.eval_state /\
+  (recorded_orac_wf f (orac_s s.eval_state).oracle ==>
+    recorded_orac_wf f (orac_s s'.eval_state).oracle)
+  )
   /\
   (! ^s env decs s' res.
   evaluate_decs s env decs = (s', res) /\
   is_record f init_s s.eval_state
   ==>
   is_record f init_s s'.eval_state /\
-  record_forward s.eval_state s'.eval_state)
+  record_forward s.eval_state s'.eval_state /\
+  (recorded_orac_wf f (orac_s s.eval_state).oracle ==>
+    recorded_orac_wf f (orac_s s'.eval_state).oracle)
+  )
 Proof
   ho_match_mp_tac terminationTheory.full_evaluate_ind
   \\ rpt conj_tac
   \\ rpt (gen_tac ORELSE disch_tac)
   \\ fs [terminationTheory.full_evaluate_def]
   \\ rveq \\ fs []
+  \\ fs [elim_Case]
   \\ simp [record_forward_refl]
+  \\ TRY (rename [`Case [App _ _]`]
+    \\ Cases_on `op = Eval` \\ Cases_on `op = Opapp` \\ fs []
+    \\ full_simp_tac bool_ss [do_eval_res_def, bool_case_eq, pair_case_eq,
+        option_case_eq, result_case_eq]
+    \\ rveq \\ full_simp_tac bool_ss [PAIR_EQ]
+    \\ rveq \\ fs []
+  )
   \\ fs [pair_case_eq, option_case_eq, result_case_eq] \\ rveq \\ fs []
+  \\ rpt (drule_then irule record_forward_trans_sym)
+  \\ simp [record_forward_refl]
   \\ fs [bool_case_eq] \\ rveq \\ fs []
   \\ simp [record_forward_refl]
   \\ fs [dec_clock_def, do_eval_res_def]
@@ -1524,16 +1571,25 @@ val agrees_impl_tac = rpt ((qpat_x_assum `orac_agrees _ _ ==> _` mp_tac
     \\ impl_tac)
   >- agrees_tac)
 
+fun simp_res_tac t = ASSUM_LIST (fn asms => let
+    val t2 = SIMP_RULE (srw_ss ()) asms t
+  in drule_then simp_res_tac t2
+    ORELSE (if is_forall (concl t) then all_tac else strip_assume_tac t)
+  end)
+
 fun imp_res_simp_tac t = IMP_RES_THEN mp_tac t
   \\ simp []
   \\ rpt ((disch_then drule \\ simp []) ORELSE disch_then
       (fn t => if is_forall (concl t) then all_tac else assume_tac t))
+
+val imp_res_simp_tac = IMP_RES_THEN simp_res_tac
 
 val insert_oracle_correct_setup = setup (
   `(! ^s env exps s' res.
   evaluate s env exps = (s', res) /\
   is_record f init_s s.eval_state /\
   orac_agrees orac s'.eval_state /\
+  orac_extended_wf f orac /\
   Case (Let, exps) /\
   res <> Rerr (Rabort Rtype_error)
   ==>
@@ -1545,6 +1601,7 @@ val insert_oracle_correct_setup = setup (
   evaluate_match s env x pes err_x = (s', res) /\
   is_record f init_s s.eval_state /\
   orac_agrees orac s'.eval_state /\
+  orac_extended_wf f orac /\
   Case (Mat, pes) /\
   res <> Rerr (Rabort Rtype_error)
   ==>
@@ -1557,6 +1614,7 @@ val insert_oracle_correct_setup = setup (
   evaluate_decs s env decs = (s', res) /\
   is_record f init_s s.eval_state /\
   orac_agrees orac s'.eval_state /\
+  orac_extended_wf f orac /\
   Case (Dlet, decs) /\
   res <> Rerr (Rabort Rtype_error)
   ==>
@@ -1571,6 +1629,9 @@ val insert_oracle_correct_setup = setup (
   \\ rveq \\ fs []
   );
 
+Triviality evaluate_is_record_forward2 =
+  evaluate_is_record_forward |> REWRITE_RULE [elim_Case]
+
 Triviality insert_oracle_correct_App:
   ^(#get_goal insert_oracle_correct_setup `Case (_, [App _ _])`)
 Proof
@@ -1582,7 +1643,7 @@ Proof
     eval_cases_tac
     \\ fs [Q.ISPEC `(a, b)` EQ_SYM_EQ] \\ rveq \\ fs []
     \\ fs [dec_clock_def]
-    \\ imp_res_simp_tac evaluate_is_record_forward
+    \\ imp_res_simp_tac evaluate_is_record_forward2
     \\ agrees_impl_tac
     \\ simp []
   )
@@ -1595,7 +1656,7 @@ Proof
     \\ rpt (disch_then drule)
     \\ disch_then (qspecl_then [`orac`, `init_s`, `f`] mp_tac)
     \\ rw []
-    \\ imp_res_simp_tac evaluate_is_record_forward
+    \\ imp_res_simp_tac evaluate_is_record_forward2
     \\ fs [bool_case_eq] \\ rveq \\ fs []
     >- (
       agrees_impl_tac
@@ -1606,7 +1667,7 @@ Proof
     \\ fs [result_case_eq, option_case_eq, pair_case_eq] \\ rveq \\ fs []
     \\ fs [error_result_case_eq] \\ rveq \\ fs []
     \\ fs [reset_env_generation_orac_eqs]
-    \\ imp_res_simp_tac evaluate_is_record_forward
+    \\ imp_res_simp_tac evaluate_is_record_forward2
     \\ imp_res_simp_tac insert_declare_env
     \\ agrees_impl_tac
     \\ simp [reset_env_generation_orac_eqs]
@@ -1622,6 +1683,7 @@ Proof
   rw []
   \\ fs [option_case_eq, pair_case_eq] \\ rveq \\ fs []
   \\ imp_res_simp_tac insert_declare_env
+  \\ simp []
 QED
 
 Theorem insert_oracle_correct:
@@ -1634,9 +1696,9 @@ Proof
     \\ eval_cases_tac
     \\ fs [Q.ISPEC `(a, b)` EQ_SYM_EQ, combine_dec_result_eq_Rerr]
     \\ rveq \\ fs []
-    \\ imp_res_simp_tac evaluate_is_record_forward
+    \\ imp_res_simp_tac evaluate_is_record_forward2
     \\ fs []
-    \\ imp_res_simp_tac evaluate_is_record_forward
+    \\ imp_res_simp_tac evaluate_is_record_forward2
     \\ agrees_impl_tac
     \\ simp []
   ) \\ NO_TAC)
@@ -1727,10 +1789,10 @@ Proof
   \\ eval_cases_tac
   \\ fs [Q.ISPEC `(a, b)` EQ_SYM_EQ, dec_clock_def]
   \\ rveq \\ fs []
-  \\ imp_res_simp_tac evaluate_is_record_forward
+  \\ imp_res_simp_tac evaluate_is_record_forward2
   \\ fs []
   \\ TRY (drule_then imp_res_simp_tac insert_do_eval \\ fs [])
-  \\ imp_res_simp_tac evaluate_is_record_forward
+  \\ imp_res_simp_tac evaluate_is_record_forward2
   \\ fs []
   \\ TRY (drule_then imp_res_simp_tac insert_declare_env)
   \\ TRY (drule_then (drule_then assume_tac) less_sub_1_cases \\ fs [])
@@ -1746,8 +1808,9 @@ QED
    source and record oracle events. Each oracle position will be a
    recorded event, if there exists a sufficient clock input so that
    enough events are recorded. The oracle is padded out with dummy
-   data, using the compiler or various backup strategies which may
-   be provided to make the dummy data more well-formed. *)
+   data, using an additional compiler (which for proof purposes may
+   be set up to succeed in cases where the real compiler may fail).
+*)
 Definition mk_eval_oracle_def:
   mk_eval_oracle compiler st0 s env decs n =
     case (OLEAST k. ?s' res.
@@ -1758,8 +1821,9 @@ Definition mk_eval_oracle_def:
         then ((0, 0), st0, [])
         else let (env_id, s_v, decs) = mk_eval_oracle compiler st0 s
                 env decs (n - 1) in
-            let (s_v2, _, _) = compiler (env_id, s_v, decs) in
-            ((0, 0), s_v2, [])
+            (case compiler (env_id, s_v, decs) of
+              | (s_v2, _, _) => ((0, 0), s_v2, [])
+            )
     | SOME k =>
       let (s', _) = evaluate_decs (s with clock := k) env decs in
         (orac_s s'.eval_state).oracle (n + 1)
@@ -1786,7 +1850,7 @@ Proof
     \\ disch_then drule
     \\ rw []
     \\ fs []
-    \\ imp_res_simp_tac evaluate_is_record_forward
+    \\ imp_res_simp_tac evaluate_is_record_forward2
     \\ fs [record_forward_def]
     \\ imp_res_tac is_record_IMP
     \\ fs []
@@ -1799,7 +1863,7 @@ Proof
     \\ disch_then drule
     \\ rw []
     \\ fs []
-    \\ imp_res_simp_tac evaluate_is_record_forward
+    \\ imp_res_simp_tac evaluate_is_record_forward2
     \\ fs [record_forward_def]
     \\ imp_res_tac is_record_IMP
     \\ fs []
@@ -1815,7 +1879,7 @@ Proof
   \\ `is_record init_eds.compiler init_eds.compiler_state
         (SOME (EvalOracle orac_s'))`
     by (simp [is_record_def] )
-  \\ imp_res_simp_tac evaluate_is_record_forward
+  \\ imp_res_simp_tac evaluate_is_record_forward2
   \\ imp_res_simp_tac is_record_IMP
   \\ fs []
   \\ rw []
@@ -1839,6 +1903,41 @@ Proof
   )
 QED
 
+Theorem mk_eval_oracle_extended_wf:
+  s_rel init_eds s t /\
+  (! args res. comp_f args = SOME res ==> FST res (FST (comp_f2 args))) /\
+  (! n t' res. evaluate_decs (t with clock := n) env decs = (t', res) ==>
+    recorded_orac_wf comp_f (orac_s t'.eval_state).oracle)
+  ==>
+  orac_extended_wf comp_f (mk_eval_oracle comp_f2 st0 t env decs)
+Proof
+  rw [orac_extended_wf_def]
+  \\ simp [Once mk_eval_oracle_def]
+  \\ DEEP_INTRO_TAC whileTheory.OLEAST_INTRO
+  \\ rw []
+  >- (
+    rpt (pairarg_tac \\ fs [])
+    \\ res_tac
+    \\ simp []
+    \\ every_case_tac
+    \\ simp []
+  )
+  >- (
+    `orac_agrees (mk_eval_oracle comp_f2 st0 t env decs) s'.eval_state`
+      by ( metis_tac [mk_eval_oracle_agrees] )
+    \\ fs [orac_agrees_def]
+    \\ every_case_tac \\ fs []
+    \\ first_x_assum (fn t => drule t
+        \\ CHANGED_TAC (simp [recorded_orac_wf_def]))
+    \\ rw []
+    \\ first_x_assum drule
+    \\ simp [ADD1]
+  )
+QED
+
+(* Creates extra oracle data like mk_eval_oracle, but without any
+   attempt to start with genuine recorded data.
+*)
 Definition mk_dummy_orac_def:
   mk_dummy_orac compiler st0 (0 : num) =
     (((0, 0), st0, []) : compiler_args) /\
@@ -1903,7 +2002,11 @@ Theorem evaluate_prog_with_clock_mk_orac_st:
   res <> Rerr (Rabort Rtype_error) /\
   init_eval_state s1.eval_state /\
   s1.refs = [] /\
-  nsAll (K concrete_v) env.v ==>
+  nsAll (K concrete_v) env.v /\
+  (case s1.eval_state of SOME (EvalDecs eds) =>
+    (! args res. eds.compiler args = SOME res ==> FST res (FST (c args)))
+    | _ => T)
+  ==>
   ?res'.
   evaluate_prog_with_clock
     (s1 with eval_state := mk_orac_st c st0 s1 env decs)
@@ -1924,6 +2027,8 @@ Proof
   \\ `s_rel e s1 (s1 with <| eval_state := SOME (EvalOracle orac_st) |>)`
   by ( unabbrev_all_tac
     \\ simp [s_rel_def, state_component_equality, recorded_orac_wf_def] )
+  \\ `is_record e.compiler e.compiler_state (SOME (EvalOracle orac_st))`
+    by ( fs [is_record_def, markerTheory.Abbrev_def] )
   \\ drule_then (qspec_then `k` assume_tac) s_rel_clock2
   \\ drule_then drule (List.last (CONJUNCTS eval_simulation))
   \\ simp [Case_def]
@@ -1932,17 +2037,27 @@ Proof
   \\ disch_tac \\ fs []
   \\ drule (List.last (CONJUNCTS insert_oracle_correct))
   \\ simp []
-  \\ disch_then (qsubterm_then `evaluate_decs _ _` mp_tac)
-  \\ simp [GSYM PULL_EXISTS, is_record_def]
-  \\ impl_tac >- (
-    fs [Case_def, markerTheory.Abbrev_def]
-    \\ rpt strip_tac \\ fs []
-    \\ rveq \\ fs []
-    \\ TRY (drule_then irule mk_eval_oracle_agrees)
-    \\ metis_tac []
+  \\ disch_then (drule_then (qsubterm_then `evaluate_decs _ _` mp_tac))
+  \\ simp [Case_def]
+  \\ reverse impl_tac
+  >- (
+    rw []
+    \\ fs [s_rel_def]
+    \\ imp_res_tac result_rel_IMP_cases \\ fs []
   )
-  \\ fs [s_rel_def]
-  \\ imp_res_tac result_rel_IMP_cases \\ fs []
+  \\ rpt strip_tac \\ fs []
+  >- (
+    drule_then irule mk_eval_oracle_agrees
+    \\ asm_exists_tac
+    \\ simp []
+  )
+  >- (
+    drule_then irule mk_eval_oracle_extended_wf
+    \\ rw []
+    \\ imp_res_simp_tac evaluate_is_record_forward2
+    \\ rfs [markerTheory.Abbrev_def]
+    \\ fs [recorded_orac_wf_def |> Q.SPECL [`c`, `K x`]]
+  )
 QED
 
 Theorem oracle_semantics_prog:
@@ -1950,6 +2065,9 @@ Theorem oracle_semantics_prog:
   outcome <> Fail /\
   init_eval_state s1.eval_state /\
   s1.refs = [] /\
+  (case s1.eval_state of SOME (EvalDecs eds) =>
+    (! args res. eds.compiler args = SOME res ==> FST res (FST (c args)))
+    | _ => T) /\
   nsAll (K concrete_v) env.v ==>
   semantics_prog (s1 with eval_state := mk_orac_st c st0 s1 env decs)
     env decs outcome
@@ -2020,6 +2138,7 @@ Proof
   \\ rw []
   \\ rpt (pairarg_tac \\ fs [])
   \\ rveq \\ fs []
+  \\ simp [pair_CASE_def]
   \\ Cases_on `evaluate_decs (s1 with clock := n) env decs`
   \\ drule_then (qspec_then `n` assume_tac) s_rel_clock2
   \\ drule_then drule (List.last (CONJUNCTS eval_simulation))
@@ -2060,9 +2179,11 @@ Proof
   )
 QED
 
-(* The constructed oracle is an infinite oracle where each state results from
-   the previous arguments to one of the compilers. To avoid partiality issues
-   though, there are two compilers provided, one of which must be total. *)
+(* Syntactic well-formedness of the infinite oracle, such as it is. Each
+   state is constructed by calling the compiler on the previous state.
+   However, the compiler is partial, and to construct a more well-formed
+   oracle we permit a second compiler to be supplied, which can succeed
+   more often. *)
 Theorem mk_orac_st_orac_wf:
   semantics_prog s1 env decs outcome /\
   outcome <> Fail /\
